<?xml version="1.0"?>
<rdf:RDF xmlns="http://www.semanticweb.org/maxsp/ontologies/2023/11/untitled-ontology-10/"
     xml:base="http://www.semanticweb.org/maxsp/ontologies/2023/11/untitled-ontology-10/"
     xmlns:owl="http://www.w3.org/2002/07/owl#"
     xmlns:rdf="http://www.w3.org/1999/02/22-rdf-syntax-ns#"
     xmlns:xml="http://www.w3.org/XML/1998/namespace"
     xmlns:xsd="http://www.w3.org/2001/XMLSchema#"
     xmlns:rdfs="http://www.w3.org/2000/01/rdf-schema#"
     xmlns:untitled-ontology-10="http://www.semanticweb.org/maxsp/ontologies/2023/11/untitled-ontology-10#">
    <owl:Ontology rdf:about="http://www.semanticweb.org/maxsp/ontologies/2023/11/untitled-ontology-10"/>
    


    <!-- 
    ///////////////////////////////////////////////////////////////////////////////////////
    //
    // Object Properties
    //
    ///////////////////////////////////////////////////////////////////////////////////////
     -->

    


    <!-- http://www.semanticweb.org/maxsp/ontologies/2023/11/untitled-ontology-10#interarrivalTime -->

    <owl:ObjectProperty rdf:about="http://www.semanticweb.org/maxsp/ontologies/2023/11/untitled-ontology-10#interarrivalTime">
        <rdfs:subPropertyOf rdf:resource="http://www.semanticweb.org/maxsp/ontologies/2023/11/untitled-ontology-10#workflowSpecifications"/>
        <rdfs:domain rdf:resource="http://www.semanticweb.org/maxsp/ontologies/2023/11/untitled-ontology-10#workflow"/>
    </owl:ObjectProperty>
    


    <!-- http://www.semanticweb.org/maxsp/ontologies/2023/11/untitled-ontology-10#personHasQualification -->

    <owl:ObjectProperty rdf:about="http://www.semanticweb.org/maxsp/ontologies/2023/11/untitled-ontology-10#personHasQualification">
        <rdfs:domain rdf:resource="http://www.semanticweb.org/maxsp/ontologies/2023/11/untitled-ontology-10#person"/>
        <rdfs:range rdf:resource="http://www.semanticweb.org/maxsp/ontologies/2023/11/untitled-ontology-10#qualification"/>
        <rdfs:comment>use this to link Instances of the Qualification Class to an instance of the Person class

to link multiple Qualifications to a Person simply add this property multiple times</rdfs:comment>
    </owl:ObjectProperty>
    


    <!-- http://www.semanticweb.org/maxsp/ontologies/2023/11/untitled-ontology-10#startTaskIs -->

    <owl:ObjectProperty rdf:about="http://www.semanticweb.org/maxsp/ontologies/2023/11/untitled-ontology-10#startTaskIs">
        <rdfs:subPropertyOf rdf:resource="http://www.semanticweb.org/maxsp/ontologies/2023/11/untitled-ontology-10#workflowSpecifications"/>
        <rdfs:domain rdf:resource="http://www.semanticweb.org/maxsp/ontologies/2023/11/untitled-ontology-10#workflow"/>
        <rdfs:range rdf:resource="http://www.semanticweb.org/maxsp/ontologies/2023/11/untitled-ontology-10#task"/>
    </owl:ObjectProperty>
    


    <!-- http://www.semanticweb.org/maxsp/ontologies/2023/11/untitled-ontology-10#taskHasPredecessor -->

    <owl:ObjectProperty rdf:about="http://www.semanticweb.org/maxsp/ontologies/2023/11/untitled-ontology-10#taskHasPredecessor">
        <rdfs:subPropertyOf rdf:resource="http://www.semanticweb.org/maxsp/ontologies/2023/11/untitled-ontology-10#taskSpecifications"/>
        <owl:inverseOf rdf:resource="http://www.semanticweb.org/maxsp/ontologies/2023/11/untitled-ontology-10#taskIsFollowedBy"/>
        <rdfs:domain rdf:resource="http://www.semanticweb.org/maxsp/ontologies/2023/11/untitled-ontology-10#task"/>
        <rdfs:range rdf:resource="http://www.semanticweb.org/maxsp/ontologies/2023/11/untitled-ontology-10#task"/>
        <rdfs:comment>with this link an intance of a task a to a task b to state that task a lies before task b

when modelling your workflow both directions need to be modelled, so dont only use taskIsFollowedBy, this will lead to faulty execution

in future this should be instantly modelled as edges instead of bidirectional references

use this property multiple times to link multiple tasks

this is used to reliably model paralellis in a Azyclic Directed Graph with a single root (startTask)</rdfs:comment>
    </owl:ObjectProperty>
    


    <!-- http://www.semanticweb.org/maxsp/ontologies/2023/11/untitled-ontology-10#taskIsFollowedBy -->

    <owl:ObjectProperty rdf:about="http://www.semanticweb.org/maxsp/ontologies/2023/11/untitled-ontology-10#taskIsFollowedBy">
        <rdfs:subPropertyOf rdf:resource="http://www.semanticweb.org/maxsp/ontologies/2023/11/untitled-ontology-10#taskSpecifications"/>
        <rdfs:domain rdf:resource="http://www.semanticweb.org/maxsp/ontologies/2023/11/untitled-ontology-10#task"/>
        <rdfs:range rdf:resource="http://www.semanticweb.org/maxsp/ontologies/2023/11/untitled-ontology-10#task"/>
        <rdfs:comment>with this link an intance of a task a to a task b to state that task a follows on task b

use this property multiple times to link multiple tasks</rdfs:comment>
    </owl:ObjectProperty>
    


    <!-- http://www.semanticweb.org/maxsp/ontologies/2023/11/untitled-ontology-10#taskNeedsQualification -->

    <owl:ObjectProperty rdf:about="http://www.semanticweb.org/maxsp/ontologies/2023/11/untitled-ontology-10#taskNeedsQualification">
        <rdfs:subPropertyOf rdf:resource="http://www.semanticweb.org/maxsp/ontologies/2023/11/untitled-ontology-10#taskSpecifications"/>
        <rdfs:domain rdf:resource="http://www.semanticweb.org/maxsp/ontologies/2023/11/untitled-ontology-10#task"/>
        <rdfs:range rdf:resource="http://www.semanticweb.org/maxsp/ontologies/2023/11/untitled-ontology-10#qualification"/>
        <rdfs:comment>this states which Qualifications are needed on a task for this task to be executed

currently this is only imported but not used in the simulation

add this property multiple times to link multiple Qualifications</rdfs:comment>
    </owl:ObjectProperty>
    


    <!-- http://www.semanticweb.org/maxsp/ontologies/2023/11/untitled-ontology-10#taskNeedsResource -->

    <owl:ObjectProperty rdf:about="http://www.semanticweb.org/maxsp/ontologies/2023/11/untitled-ontology-10#taskNeedsResource">
        <rdfs:subPropertyOf rdf:resource="http://www.semanticweb.org/maxsp/ontologies/2023/11/untitled-ontology-10#taskSpecifications"/>
        <rdfs:domain rdf:resource="http://www.semanticweb.org/maxsp/ontologies/2023/11/untitled-ontology-10#task"/>
        <rdfs:range rdf:resource="http://www.semanticweb.org/maxsp/ontologies/2023/11/untitled-ontology-10#resourceType"/>
        <rdfs:comment>use this to link the needed RsourceTypes on this task

use this multiple times for every Resource Type that is needed

if a task needs multiple resources of the same type, use this property multiple times, each time for every needed resource of that type</rdfs:comment>
    </owl:ObjectProperty>
    


    <!-- http://www.semanticweb.org/maxsp/ontologies/2023/11/untitled-ontology-10#taskSpecifications -->

    <owl:ObjectProperty rdf:about="http://www.semanticweb.org/maxsp/ontologies/2023/11/untitled-ontology-10#taskSpecifications"/>
    


    <!-- http://www.semanticweb.org/maxsp/ontologies/2023/11/untitled-ontology-10#workflowSpecifications -->

    <owl:ObjectProperty rdf:about="http://www.semanticweb.org/maxsp/ontologies/2023/11/untitled-ontology-10#workflowSpecifications"/>
    


    <!-- 
    ///////////////////////////////////////////////////////////////////////////////////////
    //
    // Data properties
    //
    ///////////////////////////////////////////////////////////////////////////////////////
     -->

    


    <!-- http://www.semanticweb.org/maxsp/ontologies/2023/11/untitled-ontology-10#eventHasName -->

    <owl:DatatypeProperty rdf:about="http://www.semanticweb.org/maxsp/ontologies/2023/11/untitled-ontology-10#eventHasName">
        <rdfs:subPropertyOf rdf:resource="http://www.semanticweb.org/maxsp/ontologies/2023/11/untitled-ontology-10#hasName"/>
        <rdfs:domain rdf:resource="http://www.semanticweb.org/maxsp/ontologies/2023/11/untitled-ontology-10#event"/>
        <rdfs:range rdf:resource="http://www.w3.org/2001/XMLSchema#string"/>
    </owl:DatatypeProperty>
    


    <!-- http://www.semanticweb.org/maxsp/ontologies/2023/11/untitled-ontology-10#eventHasStartTime -->

    <owl:DatatypeProperty rdf:about="http://www.semanticweb.org/maxsp/ontologies/2023/11/untitled-ontology-10#eventHasStartTime">
        <rdfs:subPropertyOf rdf:resource="http://www.semanticweb.org/maxsp/ontologies/2023/11/untitled-ontology-10#hasTimeSpecification"/>
        <rdfs:domain rdf:resource="http://www.semanticweb.org/maxsp/ontologies/2023/11/untitled-ontology-10#event"/>
        <rdfs:range rdf:resource="http://www.w3.org/2001/XMLSchema#decimal"/>
        <rdfs:comment>specify a a value for the time in seconds that this event should occur after simStart</rdfs:comment>
    </owl:DatatypeProperty>
    


    <!-- http://www.semanticweb.org/maxsp/ontologies/2023/11/untitled-ontology-10#eventPriority -->

    <owl:DatatypeProperty rdf:about="http://www.semanticweb.org/maxsp/ontologies/2023/11/untitled-ontology-10#eventPriority">
        <rdfs:subPropertyOf rdf:resource="http://www.semanticweb.org/maxsp/ontologies/2023/11/untitled-ontology-10#hasPriority"/>
        <rdfs:domain rdf:resource="http://www.semanticweb.org/maxsp/ontologies/2023/11/untitled-ontology-10#event"/>
        <rdfs:range rdf:resource="http://www.w3.org/2001/XMLSchema#decimal"/>
    </owl:DatatypeProperty>
    


    <!-- http://www.semanticweb.org/maxsp/ontologies/2023/11/untitled-ontology-10#hasName -->

    <owl:DatatypeProperty rdf:about="http://www.semanticweb.org/maxsp/ontologies/2023/11/untitled-ontology-10#hasName">
        <rdfs:range rdf:resource="http://www.w3.org/2001/XMLSchema#string"/>
        <rdfs:comment>some Name Specification, every Class has exactly one of these relations 

every instance needs a value along the proeprty of the certain class to be recognized by the importer</rdfs:comment>
    </owl:DatatypeProperty>
    


    <!-- http://www.semanticweb.org/maxsp/ontologies/2023/11/untitled-ontology-10#hasPriority -->

    <owl:DatatypeProperty rdf:about="http://www.semanticweb.org/maxsp/ontologies/2023/11/untitled-ontology-10#hasPriority">
        <rdfs:comment>some priority specification as Integer, is used to prioritize some events or tasks over others, for more information the implementation needs to be checked

when writing this these values are only used in comparators defined in the workflow class</rdfs:comment>
    </owl:DatatypeProperty>
    


    <!-- http://www.semanticweb.org/maxsp/ontologies/2023/11/untitled-ontology-10#hasTimeSpecification -->

    <owl:DatatypeProperty rdf:about="http://www.semanticweb.org/maxsp/ontologies/2023/11/untitled-ontology-10#hasTimeSpecification">
        <rdfs:comment>some time specification in seconds</rdfs:comment>
    </owl:DatatypeProperty>
    


    <!-- http://www.semanticweb.org/maxsp/ontologies/2023/11/untitled-ontology-10#interarrivalTime -->

    <owl:DatatypeProperty rdf:about="http://www.semanticweb.org/maxsp/ontologies/2023/11/untitled-ontology-10#interarrivalTime"/>
    


    <!-- http://www.semanticweb.org/maxsp/ontologies/2023/11/untitled-ontology-10#limitedNumber -->

    <owl:DatatypeProperty rdf:about="http://www.semanticweb.org/maxsp/ontologies/2023/11/untitled-ontology-10#limitedNumber">
        <rdfs:subPropertyOf rdf:resource="http://www.semanticweb.org/maxsp/ontologies/2023/11/untitled-ontology-10#resourceSpecifications"/>
        <rdfs:domain rdf:resource="http://www.semanticweb.org/maxsp/ontologies/2023/11/untitled-ontology-10#resourceType"/>
        <rdfs:range rdf:resource="http://www.w3.org/2001/XMLSchema#int"/>
        <rdfs:comment>dies bedeutet, dass beim importieren die entsprechende Anzahl an Resourcen dieses Typs erstellt wird. Ist der Ressourcen Typ zb &quot;Formular&quot; und der übergebene Integer ist 100, werden 100 Instanzen eines Formulars erstellt.

Nur ganze positive Zahlen angeben

0 für unlimitierten ResourcenZugriff</rdfs:comment>
    </owl:DatatypeProperty>
    


    <!-- http://www.semanticweb.org/maxsp/ontologies/2023/11/untitled-ontology-10#numbersOfUse -->

    <owl:DatatypeProperty rdf:about="http://www.semanticweb.org/maxsp/ontologies/2023/11/untitled-ontology-10#numbersOfUse">
        <rdfs:subPropertyOf rdf:resource="http://www.semanticweb.org/maxsp/ontologies/2023/11/untitled-ontology-10#resourceSpecifications"/>
        <rdfs:domain rdf:resource="http://www.semanticweb.org/maxsp/ontologies/2023/11/untitled-ontology-10#resourceType"/>
        <rdfs:range rdf:resource="http://www.w3.org/2001/XMLSchema#positiveInteger"/>
        <rdfs:comment>dies kann auch genutzt werden um für Resourcen des gleichen Typs unterschiedliche Werte festzulegen. Dafür muss diese Propertie an dem jeweiligen Resourcen Individuum spezifiziert werden. Ein Wert entlang dieser Property an einem Individuum Resource überschreibt für das Individuum den Wert der für den Resourcen Typen festeglegt wurde</rdfs:comment>
        <rdfs:comment>wird dies für einen resourcen Typen angegeben, wird dies für alle Resourcen des Typs angewendet, die keinen eigenen Wert für diese Propertie haben</rdfs:comment>
        <rdfs:comment>wird diese property bei resource type nicht verwendet, wird kann die erstellte Resource beliebig oft verwendet werden

eine 1 bedeutet dass die Resource nur ein einziges Mal verwendet werden kann und dann vernichtet wird (z.B. Formular)

eine 0 bedeutet dass die Resource beliebig oft verwendet werden kann z.B. (Rettungswagen), 

eine Zahl &gt; 1 gibt die Anzahl der Nutzungen für eine Resource an bevor diese nicht mehr genutzt werden kann</rdfs:comment>
    </owl:DatatypeProperty>
    


    <!-- http://www.semanticweb.org/maxsp/ontologies/2023/11/untitled-ontology-10#personHasName -->

    <owl:DatatypeProperty rdf:about="http://www.semanticweb.org/maxsp/ontologies/2023/11/untitled-ontology-10#personHasName">
        <rdfs:subPropertyOf rdf:resource="http://www.semanticweb.org/maxsp/ontologies/2023/11/untitled-ontology-10#hasName"/>
        <rdfs:domain rdf:resource="http://www.semanticweb.org/maxsp/ontologies/2023/11/untitled-ontology-10#person"/>
        <rdfs:range rdf:resource="http://www.w3.org/2001/XMLSchema#string"/>
    </owl:DatatypeProperty>
    


    <!-- http://www.semanticweb.org/maxsp/ontologies/2023/11/untitled-ontology-10#qualificationHasName -->

    <owl:DatatypeProperty rdf:about="http://www.semanticweb.org/maxsp/ontologies/2023/11/untitled-ontology-10#qualificationHasName">
        <rdfs:subPropertyOf rdf:resource="http://www.semanticweb.org/maxsp/ontologies/2023/11/untitled-ontology-10#hasName"/>
        <rdfs:domain rdf:resource="http://www.semanticweb.org/maxsp/ontologies/2023/11/untitled-ontology-10#qualification"/>
        <rdfs:range rdf:resource="http://www.w3.org/2001/XMLSchema#string"/>
    </owl:DatatypeProperty>
    


    <!-- http://www.semanticweb.org/maxsp/ontologies/2023/11/untitled-ontology-10#resourceSpecifications -->

    <owl:DatatypeProperty rdf:about="http://www.semanticweb.org/maxsp/ontologies/2023/11/untitled-ontology-10#resourceSpecifications"/>
    


    <!-- http://www.semanticweb.org/maxsp/ontologies/2023/11/untitled-ontology-10#resourceTypeHasName -->

    <owl:DatatypeProperty rdf:about="http://www.semanticweb.org/maxsp/ontologies/2023/11/untitled-ontology-10#resourceTypeHasName">
        <rdfs:subPropertyOf rdf:resource="http://www.semanticweb.org/maxsp/ontologies/2023/11/untitled-ontology-10#hasName"/>
        <rdfs:domain rdf:resource="http://www.semanticweb.org/maxsp/ontologies/2023/11/untitled-ontology-10#resourceType"/>
        <rdfs:range rdf:resource="http://www.w3.org/2001/XMLSchema#string"/>
    </owl:DatatypeProperty>
    


    <!-- http://www.semanticweb.org/maxsp/ontologies/2023/11/untitled-ontology-10#taskHasName -->

    <owl:DatatypeProperty rdf:about="http://www.semanticweb.org/maxsp/ontologies/2023/11/untitled-ontology-10#taskHasName">
        <rdfs:subPropertyOf rdf:resource="http://www.semanticweb.org/maxsp/ontologies/2023/11/untitled-ontology-10#hasName"/>
        <rdfs:domain rdf:resource="http://www.semanticweb.org/maxsp/ontologies/2023/11/untitled-ontology-10#task"/>
        <rdfs:range rdf:resource="http://www.w3.org/2001/XMLSchema#string"/>
    </owl:DatatypeProperty>
    


    <!-- http://www.semanticweb.org/maxsp/ontologies/2023/11/untitled-ontology-10#taskHasTimeNeeded -->

    <owl:DatatypeProperty rdf:about="http://www.semanticweb.org/maxsp/ontologies/2023/11/untitled-ontology-10#taskHasTimeNeeded">
        <rdfs:subPropertyOf rdf:resource="http://www.semanticweb.org/maxsp/ontologies/2023/11/untitled-ontology-10#hasTimeSpecification"/>
        <rdfs:comment>specify a value in seconds that this task takes from the start to the end of its execution</rdfs:comment>
    </owl:DatatypeProperty>
    


    <!-- http://www.semanticweb.org/maxsp/ontologies/2023/11/untitled-ontology-10#taskPriority -->

    <owl:DatatypeProperty rdf:about="http://www.semanticweb.org/maxsp/ontologies/2023/11/untitled-ontology-10#taskPriority">
        <rdfs:subPropertyOf rdf:resource="http://www.semanticweb.org/maxsp/ontologies/2023/11/untitled-ontology-10#hasPriority"/>
        <rdfs:domain rdf:resource="http://www.semanticweb.org/maxsp/ontologies/2023/11/untitled-ontology-10#task"/>
        <rdfs:range rdf:resource="http://www.w3.org/2001/XMLSchema#decimal"/>
    </owl:DatatypeProperty>
    


    <!-- http://www.semanticweb.org/maxsp/ontologies/2023/11/untitled-ontology-10#taskSpecificationDataProperty -->

    <owl:DatatypeProperty rdf:about="http://www.semanticweb.org/maxsp/ontologies/2023/11/untitled-ontology-10#taskSpecificationDataProperty"/>
    


    <!-- http://www.semanticweb.org/maxsp/ontologies/2023/11/untitled-ontology-10#workflowHasName -->

    <owl:DatatypeProperty rdf:about="http://www.semanticweb.org/maxsp/ontologies/2023/11/untitled-ontology-10#workflowHasName">
        <rdfs:subPropertyOf rdf:resource="http://www.semanticweb.org/maxsp/ontologies/2023/11/untitled-ontology-10#hasName"/>
        <rdfs:domain rdf:resource="http://www.semanticweb.org/maxsp/ontologies/2023/11/untitled-ontology-10#workflow"/>
        <rdfs:range rdf:resource="http://www.w3.org/2001/XMLSchema#string"/>
    </owl:DatatypeProperty>
    


    <!-- http://www.semanticweb.org/maxsp/ontologies/2023/11/untitled-ontology-10#workflowSpecifications -->

    <owl:DatatypeProperty rdf:about="http://www.semanticweb.org/maxsp/ontologies/2023/11/untitled-ontology-10#workflowSpecifications"/>
    


    <!-- 
    ///////////////////////////////////////////////////////////////////////////////////////
    //
    // Classes
    //
    ///////////////////////////////////////////////////////////////////////////////////////
     -->

    


    <!-- http://www.semanticweb.org/maxsp/ontologies/2023/11/untitled-ontology-10#event -->

    <owl:Class rdf:about="http://www.semanticweb.org/maxsp/ontologies/2023/11/untitled-ontology-10#event">
        <rdfs:comment>a class for the events that cycle from start to endTasks

any instance of this cclass needs the name property to be recognized by the importer

also required is the startTime and the priority property

as currently only one workflow is supported, every event will be scheduled to this workflow at the specified startTime</rdfs:comment>
    </owl:Class>
    


    <!-- http://www.semanticweb.org/maxsp/ontologies/2023/11/untitled-ontology-10#person -->

    <owl:Class rdf:about="http://www.semanticweb.org/maxsp/ontologies/2023/11/untitled-ontology-10#person">
        <rdfs:comment>a class for persons, every instance needs the name property to be recognized by the importer

there is the personHasQualification property to link Qualifications to Persons

persons do get imported but the use is not implemented in simulation and is a TODO</rdfs:comment>
    </owl:Class>
    


    <!-- http://www.semanticweb.org/maxsp/ontologies/2023/11/untitled-ontology-10#qualification -->

    <owl:Class rdf:about="http://www.semanticweb.org/maxsp/ontologies/2023/11/untitled-ontology-10#qualification">
        <rdfs:comment>a qualification is something a person needs to have to be capable of working on a task that requires certain qualifications. you need to have the name property for every instance for the importer to recognize instances of this class

currently this is not implemented, but the necessary proeprties to add this to a task are given via taskHasQualification.</rdfs:comment>
    </owl:Class>
    


    <!-- http://www.semanticweb.org/maxsp/ontologies/2023/11/untitled-ontology-10#resourceType -->

    <owl:Class rdf:about="http://www.semanticweb.org/maxsp/ontologies/2023/11/untitled-ontology-10#resourceType">
        <rdfs:comment>this is used to specify resources of a certain type. it needs the name property for this class at least to be recognized by the importer
with no further specfications this this resource tpe is treated as descirbing a unlimited resourcetype
you can specify limitedNumber property with a int &gt; 0 and there will be this number of resources created of this type
specify numberOfUse with a int &gt; 0 and a resource can be used this certain amount of time (not implemented yet)</rdfs:comment>
    </owl:Class>
    


    <!-- http://www.semanticweb.org/maxsp/ontologies/2023/11/untitled-ontology-10#task -->

    <owl:Class rdf:about="http://www.semanticweb.org/maxsp/ontologies/2023/11/untitled-ontology-10#task">
        <rdfs:comment>this is a class for the tasks

any instance needs the name property to be recognized by the importer

also required are the properties taskTimeNeeded, taskPriority

a task can have multiple isFollowedBy hasPredecessor, hasQualification needs Resource.

if no followed By or has Predecessor the task is not part of a workflow, as there is no connection
if no followedBy, this is a endTask
if no hasPredecessor this is a startTask

there can be only one startTask in one workflow at this time so multiple task with no predecessor will result in errors

to specify that there are multiple resources, qualification needed or tasks linked, use the certain property multiple times and link the instances</rdfs:comment>
    </owl:Class>
    


    <!-- http://www.semanticweb.org/maxsp/ontologies/2023/11/untitled-ontology-10#workflow -->

    <owl:Class rdf:about="http://www.semanticweb.org/maxsp/ontologies/2023/11/untitled-ontology-10#workflow">
        <rdfs:comment>this is a class for the workflows

any instance of this class needs the name property to be recognized by the importer

also you need to provide a link to the start task

currently only one workflow is supported, so do not add multiple instances of the workflow unless you checked the implementation</rdfs:comment>
    </owl:Class>
    


    <!-- 
    ///////////////////////////////////////////////////////////////////////////////////////
    //
    // Individuals
    //
    ///////////////////////////////////////////////////////////////////////////////////////
     -->

    


    <!-- http://www.semanticweb.org/maxsp/ontologies/2023/11/untitled-ontology-10#Event:event1 -->

    <owl:NamedIndividual rdf:about="http://www.semanticweb.org/maxsp/ontologies/2023/11/untitled-ontology-10#Event:event1">
        <rdf:type rdf:resource="http://www.semanticweb.org/maxsp/ontologies/2023/11/untitled-ontology-10#event"/>
        <untitled-ontology-10:eventHasName>event1</untitled-ontology-10:eventHasName>
        <untitled-ontology-10:eventHasStartTime rdf:datatype="http://www.w3.org/2001/XMLSchema#decimal">5</untitled-ontology-10:eventHasStartTime>
        <untitled-ontology-10:eventPriority rdf:datatype="http://www.w3.org/2001/XMLSchema#decimal">1</untitled-ontology-10:eventPriority>
    </owl:NamedIndividual>
    


    <!-- http://www.semanticweb.org/maxsp/ontologies/2023/11/untitled-ontology-10#Event:event2 -->

    <owl:NamedIndividual rdf:about="http://www.semanticweb.org/maxsp/ontologies/2023/11/untitled-ontology-10#Event:event2">
        <rdf:type rdf:resource="http://www.semanticweb.org/maxsp/ontologies/2023/11/untitled-ontology-10#event"/>
        <untitled-ontology-10:eventHasName>event2</untitled-ontology-10:eventHasName>
        <untitled-ontology-10:eventHasStartTime rdf:datatype="http://www.w3.org/2001/XMLSchema#decimal">7</untitled-ontology-10:eventHasStartTime>
        <untitled-ontology-10:eventPriority rdf:datatype="http://www.w3.org/2001/XMLSchema#decimal">1</untitled-ontology-10:eventPriority>
    </owl:NamedIndividual>
    


    <!-- http://www.semanticweb.org/maxsp/ontologies/2023/11/untitled-ontology-10#Event:event3 -->

    <owl:NamedIndividual rdf:about="http://www.semanticweb.org/maxsp/ontologies/2023/11/untitled-ontology-10#Event:event3">
        <rdf:type rdf:resource="http://www.semanticweb.org/maxsp/ontologies/2023/11/untitled-ontology-10#event"/>
        <untitled-ontology-10:eventHasName>event3</untitled-ontology-10:eventHasName>
        <untitled-ontology-10:eventHasStartTime rdf:datatype="http://www.w3.org/2001/XMLSchema#decimal">10</untitled-ontology-10:eventHasStartTime>
        <untitled-ontology-10:eventPriority rdf:datatype="http://www.w3.org/2001/XMLSchema#decimal">2</untitled-ontology-10:eventPriority>
    </owl:NamedIndividual>
    


    <!-- http://www.semanticweb.org/maxsp/ontologies/2023/11/untitled-ontology-10#Event:event4 -->

    <owl:NamedIndividual rdf:about="http://www.semanticweb.org/maxsp/ontologies/2023/11/untitled-ontology-10#Event:event4">
        <rdf:type rdf:resource="http://www.semanticweb.org/maxsp/ontologies/2023/11/untitled-ontology-10#event"/>
        <untitled-ontology-10:eventHasName>event4</untitled-ontology-10:eventHasName>
        <untitled-ontology-10:eventHasStartTime rdf:datatype="http://www.w3.org/2001/XMLSchema#decimal">25</untitled-ontology-10:eventHasStartTime>
        <untitled-ontology-10:eventPriority rdf:datatype="http://www.w3.org/2001/XMLSchema#decimal">1</untitled-ontology-10:eventPriority>
    </owl:NamedIndividual>
    


    <!-- http://www.semanticweb.org/maxsp/ontologies/2023/11/untitled-ontology-10#Qualification:Counsellor -->

    <owl:NamedIndividual rdf:about="http://www.semanticweb.org/maxsp/ontologies/2023/11/untitled-ontology-10#Qualification:Counsellor">
        <rdf:type rdf:resource="http://www.semanticweb.org/maxsp/ontologies/2023/11/untitled-ontology-10#qualification"/>
        <untitled-ontology-10:qualificationHasName>Counsellor</untitled-ontology-10:qualificationHasName>
    </owl:NamedIndividual>
    


    <!-- http://www.semanticweb.org/maxsp/ontologies/2023/11/untitled-ontology-10#Qualification:Doctor -->

    <owl:NamedIndividual rdf:about="http://www.semanticweb.org/maxsp/ontologies/2023/11/untitled-ontology-10#Qualification:Doctor">
        <rdf:type rdf:resource="http://www.semanticweb.org/maxsp/ontologies/2023/11/untitled-ontology-10#qualification"/>
        <untitled-ontology-10:qualificationHasName>Doctor</untitled-ontology-10:qualificationHasName>
    </owl:NamedIndividual>
    


    <!-- http://www.semanticweb.org/maxsp/ontologies/2023/11/untitled-ontology-10#Qualification:Lab_technician -->

    <owl:NamedIndividual rdf:about="http://www.semanticweb.org/maxsp/ontologies/2023/11/untitled-ontology-10#Qualification:Lab_technician">
        <rdf:type rdf:resource="http://www.semanticweb.org/maxsp/ontologies/2023/11/untitled-ontology-10#qualification"/>
        <untitled-ontology-10:qualificationHasName>Lab_technician</untitled-ontology-10:qualificationHasName>
    </owl:NamedIndividual>
    


    <!-- http://www.semanticweb.org/maxsp/ontologies/2023/11/untitled-ontology-10#Qualification:Nurse -->

    <owl:NamedIndividual rdf:about="http://www.semanticweb.org/maxsp/ontologies/2023/11/untitled-ontology-10#Qualification:Nurse">
        <rdf:type rdf:resource="http://www.semanticweb.org/maxsp/ontologies/2023/11/untitled-ontology-10#qualification"/>
        <untitled-ontology-10:qualificationHasName>Nurse</untitled-ontology-10:qualificationHasName>
    </owl:NamedIndividual>
    


    <!-- http://www.semanticweb.org/maxsp/ontologies/2023/11/untitled-ontology-10#ResourceType:AdmissionDetails -->

    <owl:NamedIndividual rdf:about="http://www.semanticweb.org/maxsp/ontologies/2023/11/untitled-ontology-10#ResourceType:AdmissionDetails">
        <rdf:type rdf:resource="http://www.semanticweb.org/maxsp/ontologies/2023/11/untitled-ontology-10#resourceType"/>
        <untitled-ontology-10:resourceTypeHasName>AdmissionDetails</untitled-ontology-10:resourceTypeHasName>
    </owl:NamedIndividual>
    


    <!-- http://www.semanticweb.org/maxsp/ontologies/2023/11/untitled-ontology-10#ResourceType:AllergyDetails -->

    <owl:NamedIndividual rdf:about="http://www.semanticweb.org/maxsp/ontologies/2023/11/untitled-ontology-10#ResourceType:AllergyDetails">
        <rdf:type rdf:resource="http://www.semanticweb.org/maxsp/ontologies/2023/11/untitled-ontology-10#resourceType"/>
        <untitled-ontology-10:resourceTypeHasName>Allergy details</untitled-ontology-10:resourceTypeHasName>
    </owl:NamedIndividual>
    


    <!-- http://www.semanticweb.org/maxsp/ontologies/2023/11/untitled-ontology-10#ResourceType:Consent_form -->

    <owl:NamedIndividual rdf:about="http://www.semanticweb.org/maxsp/ontologies/2023/11/untitled-ontology-10#ResourceType:Consent_form">
        <rdf:type rdf:resource="http://www.semanticweb.org/maxsp/ontologies/2023/11/untitled-ontology-10#resourceType"/>
        <untitled-ontology-10:resourceTypeHasName>Consent_form</untitled-ontology-10:resourceTypeHasName>
    </owl:NamedIndividual>
    


    <!-- http://www.semanticweb.org/maxsp/ontologies/2023/11/untitled-ontology-10#ResourceType:Diet_Details -->

    <owl:NamedIndividual rdf:about="http://www.semanticweb.org/maxsp/ontologies/2023/11/untitled-ontology-10#ResourceType:Diet_Details">
        <rdf:type rdf:resource="http://www.semanticweb.org/maxsp/ontologies/2023/11/untitled-ontology-10#resourceType"/>
        <untitled-ontology-10:resourceTypeHasName>Diet_Details</untitled-ontology-10:resourceTypeHasName>
    </owl:NamedIndividual>
    


    <!-- http://www.semanticweb.org/maxsp/ontologies/2023/11/untitled-ontology-10#ResourceType:Lab_test -->

    <owl:NamedIndividual rdf:about="http://www.semanticweb.org/maxsp/ontologies/2023/11/untitled-ontology-10#ResourceType:Lab_test">
        <rdf:type rdf:resource="http://www.semanticweb.org/maxsp/ontologies/2023/11/untitled-ontology-10#resourceType"/>
        <untitled-ontology-10:resourceTypeHasName>Lab_test</untitled-ontology-10:resourceTypeHasName>
    </owl:NamedIndividual>
    


    <!-- http://www.semanticweb.org/maxsp/ontologies/2023/11/untitled-ontology-10#ResourceType:PatientsDetails -->

    <owl:NamedIndividual rdf:about="http://www.semanticweb.org/maxsp/ontologies/2023/11/untitled-ontology-10#ResourceType:PatientsDetails">
        <rdf:type rdf:resource="http://www.semanticweb.org/maxsp/ontologies/2023/11/untitled-ontology-10#resourceType"/>
        <untitled-ontology-10:resourceTypeHasName>Patient&apos;s details</untitled-ontology-10:resourceTypeHasName>
    </owl:NamedIndividual>
    


    <!-- http://www.semanticweb.org/maxsp/ontologies/2023/11/untitled-ontology-10#ResourceType:Patients_file -->

    <owl:NamedIndividual rdf:about="http://www.semanticweb.org/maxsp/ontologies/2023/11/untitled-ontology-10#ResourceType:Patients_file">
        <rdf:type rdf:resource="http://www.semanticweb.org/maxsp/ontologies/2023/11/untitled-ontology-10#resourceType"/>
        <untitled-ontology-10:resourceTypeHasName>Patient&apos;s file</untitled-ontology-10:resourceTypeHasName>
    </owl:NamedIndividual>
    


    <!-- http://www.semanticweb.org/maxsp/ontologies/2023/11/untitled-ontology-10#ResourceType:Present_medications -->

    <owl:NamedIndividual rdf:about="http://www.semanticweb.org/maxsp/ontologies/2023/11/untitled-ontology-10#ResourceType:Present_medications">
        <rdf:type rdf:resource="http://www.semanticweb.org/maxsp/ontologies/2023/11/untitled-ontology-10#resourceType"/>
        <untitled-ontology-10:resourceTypeHasName>Present medications</untitled-ontology-10:resourceTypeHasName>
    </owl:NamedIndividual>
    


    <!-- http://www.semanticweb.org/maxsp/ontologies/2023/11/untitled-ontology-10#ResourceType:Signed_form -->

    <owl:NamedIndividual rdf:about="http://www.semanticweb.org/maxsp/ontologies/2023/11/untitled-ontology-10#ResourceType:Signed_form">
        <rdf:type rdf:resource="http://www.semanticweb.org/maxsp/ontologies/2023/11/untitled-ontology-10#resourceType"/>
        <untitled-ontology-10:resourceTypeHasName>Signed_form</untitled-ontology-10:resourceTypeHasName>
    </owl:NamedIndividual>
    


    <!-- http://www.semanticweb.org/maxsp/ontologies/2023/11/untitled-ontology-10#ResourceType:Stethoscope -->

    <owl:NamedIndividual rdf:about="http://www.semanticweb.org/maxsp/ontologies/2023/11/untitled-ontology-10#ResourceType:Stethoscope">
        <rdf:type rdf:resource="http://www.semanticweb.org/maxsp/ontologies/2023/11/untitled-ontology-10#resourceType"/>
        <untitled-ontology-10:limitedNumber rdf:datatype="http://www.w3.org/2001/XMLSchema#decimal">1</untitled-ontology-10:limitedNumber>
        <untitled-ontology-10:resourceTypeHasName>Stethoscope</untitled-ontology-10:resourceTypeHasName>
    </owl:NamedIndividual>
    


    <!-- http://www.semanticweb.org/maxsp/ontologies/2023/11/untitled-ontology-10#ResourceType:Surgical_dress -->

    <owl:NamedIndividual rdf:about="http://www.semanticweb.org/maxsp/ontologies/2023/11/untitled-ontology-10#ResourceType:Surgical_dress">
        <rdf:type rdf:resource="http://www.semanticweb.org/maxsp/ontologies/2023/11/untitled-ontology-10#resourceType"/>
        <untitled-ontology-10:resourceTypeHasName>Surgical_dress</untitled-ontology-10:resourceTypeHasName>
    </owl:NamedIndividual>
    


    <!-- http://www.semanticweb.org/maxsp/ontologies/2023/11/untitled-ontology-10#ResourceType:X-ray_machine -->

    <owl:NamedIndividual rdf:about="http://www.semanticweb.org/maxsp/ontologies/2023/11/untitled-ontology-10#ResourceType:X-ray_machine">
        <rdf:type rdf:resource="http://www.semanticweb.org/maxsp/ontologies/2023/11/untitled-ontology-10#resourceType"/>
        <untitled-ontology-10:limitedNumber rdf:datatype="http://www.w3.org/2001/XMLSchema#decimal">1</untitled-ontology-10:limitedNumber>
        <untitled-ontology-10:resourceTypeHasName>X-ray_machine</untitled-ontology-10:resourceTypeHasName>
    </owl:NamedIndividual>
    


    <!-- http://www.semanticweb.org/maxsp/ontologies/2023/11/untitled-ontology-10#Task:Instruction_to_Patient -->

    <owl:NamedIndividual rdf:about="http://www.semanticweb.org/maxsp/ontologies/2023/11/untitled-ontology-10#Task:Instruction_to_Patient">
        <rdf:type rdf:resource="http://www.semanticweb.org/maxsp/ontologies/2023/11/untitled-ontology-10#task"/>
        <untitled-ontology-10:taskHasPredecessor rdf:resource="http://www.semanticweb.org/maxsp/ontologies/2023/11/untitled-ontology-10#Task:Medical_examination"/>
        <untitled-ontology-10:taskIsFollowedBy rdf:resource="http://www.semanticweb.org/maxsp/ontologies/2023/11/untitled-ontology-10#Task:Pre-operative_test"/>
        <untitled-ontology-10:taskNeedsQualification rdf:resource="http://www.semanticweb.org/maxsp/ontologies/2023/11/untitled-ontology-10#Qualification:Nurse"/>
        <untitled-ontology-10:taskNeedsResource rdf:resource="http://www.semanticweb.org/maxsp/ontologies/2023/11/untitled-ontology-10#ResourceType:AdmissionDetails"/>
        <untitled-ontology-10:taskNeedsResource rdf:resource="http://www.semanticweb.org/maxsp/ontologies/2023/11/untitled-ontology-10#ResourceType:Diet_Details"/>
        <untitled-ontology-10:taskNeedsResource rdf:resource="http://www.semanticweb.org/maxsp/ontologies/2023/11/untitled-ontology-10#ResourceType:Stethoscope"/>
        <untitled-ontology-10:taskHasName>Instruction_to_Patient</untitled-ontology-10:taskHasName>
        <untitled-ontology-10:taskHasTimeNeeded rdf:datatype="http://www.w3.org/2001/XMLSchema#decimal">10</untitled-ontology-10:taskHasTimeNeeded>
        <untitled-ontology-10:taskPriority rdf:datatype="http://www.w3.org/2001/XMLSchema#decimal">1</untitled-ontology-10:taskPriority>
    </owl:NamedIndividual>
    


    <!-- http://www.semanticweb.org/maxsp/ontologies/2023/11/untitled-ontology-10#Task:Medical_examination -->

    <owl:NamedIndividual rdf:about="http://www.semanticweb.org/maxsp/ontologies/2023/11/untitled-ontology-10#Task:Medical_examination">
        <rdf:type rdf:resource="http://www.semanticweb.org/maxsp/ontologies/2023/11/untitled-ontology-10#task"/>
        <untitled-ontology-10:taskIsFollowedBy rdf:resource="http://www.semanticweb.org/maxsp/ontologies/2023/11/untitled-ontology-10#Task:Instruction_to_Patient"/>
        <untitled-ontology-10:taskIsFollowedBy rdf:resource="http://www.semanticweb.org/maxsp/ontologies/2023/11/untitled-ontology-10#Task:Reviewing_Patient_History"/>
        <untitled-ontology-10:taskNeedsQualification rdf:resource="http://www.semanticweb.org/maxsp/ontologies/2023/11/untitled-ontology-10#Qualification:Doctor"/>
        <untitled-ontology-10:taskNeedsResource rdf:resource="http://www.semanticweb.org/maxsp/ontologies/2023/11/untitled-ontology-10#ResourceType:Stethoscope"/>
        <untitled-ontology-10:taskHasName>Medical_examination</untitled-ontology-10:taskHasName>
        <untitled-ontology-10:taskHasTimeNeeded rdf:datatype="http://www.w3.org/2001/XMLSchema#decimal">15</untitled-ontology-10:taskHasTimeNeeded>
        <untitled-ontology-10:taskPriority rdf:datatype="http://www.w3.org/2001/XMLSchema#decimal">1</untitled-ontology-10:taskPriority>
    </owl:NamedIndividual>
    


    <!-- http://www.semanticweb.org/maxsp/ontologies/2023/11/untitled-ontology-10#Task:Patient_preparation -->

    <owl:NamedIndividual rdf:about="http://www.semanticweb.org/maxsp/ontologies/2023/11/untitled-ontology-10#Task:Patient_preparation">
        <rdf:type rdf:resource="http://www.semanticweb.org/maxsp/ontologies/2023/11/untitled-ontology-10#task"/>
        <untitled-ontology-10:taskHasPredecessor rdf:resource="http://www.semanticweb.org/maxsp/ontologies/2023/11/untitled-ontology-10#Task:Pre-operative_Counselling_and_Consent"/>
        <untitled-ontology-10:taskNeedsQualification rdf:resource="http://www.semanticweb.org/maxsp/ontologies/2023/11/untitled-ontology-10#Qualification:Nurse"/>
        <untitled-ontology-10:taskNeedsResource rdf:resource="http://www.semanticweb.org/maxsp/ontologies/2023/11/untitled-ontology-10#ResourceType:Surgical_dress"/>
        <untitled-ontology-10:taskHasName>Patient_preparation</untitled-ontology-10:taskHasName>
        <untitled-ontology-10:taskHasTimeNeeded rdf:datatype="http://www.w3.org/2001/XMLSchema#decimal">10</untitled-ontology-10:taskHasTimeNeeded>
        <untitled-ontology-10:taskPriority rdf:datatype="http://www.w3.org/2001/XMLSchema#decimal">1</untitled-ontology-10:taskPriority>
    </owl:NamedIndividual>
    


    <!-- http://www.semanticweb.org/maxsp/ontologies/2023/11/untitled-ontology-10#Task:Pre-operative_Counselling_and_Consent -->

    <owl:NamedIndividual rdf:about="http://www.semanticweb.org/maxsp/ontologies/2023/11/untitled-ontology-10#Task:Pre-operative_Counselling_and_Consent">
        <rdf:type rdf:resource="http://www.semanticweb.org/maxsp/ontologies/2023/11/untitled-ontology-10#task"/>
        <untitled-ontology-10:taskHasPredecessor rdf:resource="http://www.semanticweb.org/maxsp/ontologies/2023/11/untitled-ontology-10#Task:Pre-operative_test"/>
        <untitled-ontology-10:taskHasPredecessor rdf:resource="http://www.semanticweb.org/maxsp/ontologies/2023/11/untitled-ontology-10#Task:Reviewing_Patient_History"/>
        <untitled-ontology-10:taskIsFollowedBy rdf:resource="http://www.semanticweb.org/maxsp/ontologies/2023/11/untitled-ontology-10#Task:Patient_preparation"/>
        <untitled-ontology-10:taskNeedsQualification rdf:resource="http://www.semanticweb.org/maxsp/ontologies/2023/11/untitled-ontology-10#Qualification:Counsellor"/>
        <untitled-ontology-10:taskNeedsResource rdf:resource="http://www.semanticweb.org/maxsp/ontologies/2023/11/untitled-ontology-10#ResourceType:Consent_form"/>
        <untitled-ontology-10:taskNeedsResource rdf:resource="http://www.semanticweb.org/maxsp/ontologies/2023/11/untitled-ontology-10#ResourceType:Signed_form"/>
        <untitled-ontology-10:taskHasName>Pre-operative_Counselling_and_Consent</untitled-ontology-10:taskHasName>
        <untitled-ontology-10:taskHasTimeNeeded rdf:datatype="http://www.w3.org/2001/XMLSchema#decimal">15</untitled-ontology-10:taskHasTimeNeeded>
        <untitled-ontology-10:taskPriority rdf:datatype="http://www.w3.org/2001/XMLSchema#decimal">1</untitled-ontology-10:taskPriority>
    </owl:NamedIndividual>
    


    <!-- http://www.semanticweb.org/maxsp/ontologies/2023/11/untitled-ontology-10#Task:Pre-operative_test -->

    <owl:NamedIndividual rdf:about="http://www.semanticweb.org/maxsp/ontologies/2023/11/untitled-ontology-10#Task:Pre-operative_test">
        <rdf:type rdf:resource="http://www.semanticweb.org/maxsp/ontologies/2023/11/untitled-ontology-10#task"/>
        <untitled-ontology-10:taskHasPredecessor rdf:resource="http://www.semanticweb.org/maxsp/ontologies/2023/11/untitled-ontology-10#Task:Instruction_to_Patient"/>
        <untitled-ontology-10:taskIsFollowedBy rdf:resource="http://www.semanticweb.org/maxsp/ontologies/2023/11/untitled-ontology-10#Task:Pre-operative_Counselling_and_Consent"/>
        <untitled-ontology-10:taskNeedsQualification rdf:resource="http://www.semanticweb.org/maxsp/ontologies/2023/11/untitled-ontology-10#Qualification:Lab_technician"/>
        <untitled-ontology-10:taskNeedsQualification rdf:resource="http://www.semanticweb.org/maxsp/ontologies/2023/11/untitled-ontology-10#Qualification:Nurse"/>
        <untitled-ontology-10:taskNeedsResource rdf:resource="http://www.semanticweb.org/maxsp/ontologies/2023/11/untitled-ontology-10#ResourceType:Lab_test"/>
        <untitled-ontology-10:taskNeedsResource rdf:resource="http://www.semanticweb.org/maxsp/ontologies/2023/11/untitled-ontology-10#ResourceType:X-ray_machine"/>
        <untitled-ontology-10:taskHasName>Pre-operative_test</untitled-ontology-10:taskHasName>
        <untitled-ontology-10:taskHasTimeNeeded rdf:datatype="http://www.w3.org/2001/XMLSchema#decimal">15</untitled-ontology-10:taskHasTimeNeeded>
        <untitled-ontology-10:taskPriority rdf:datatype="http://www.w3.org/2001/XMLSchema#decimal">1</untitled-ontology-10:taskPriority>
    </owl:NamedIndividual>
    


    <!-- http://www.semanticweb.org/maxsp/ontologies/2023/11/untitled-ontology-10#Task:Reviewing_Patient_History -->

    <owl:NamedIndividual rdf:about="http://www.semanticweb.org/maxsp/ontologies/2023/11/untitled-ontology-10#Task:Reviewing_Patient_History">
        <rdf:type rdf:resource="http://www.semanticweb.org/maxsp/ontologies/2023/11/untitled-ontology-10#task"/>
        <untitled-ontology-10:taskHasPredecessor rdf:resource="http://www.semanticweb.org/maxsp/ontologies/2023/11/untitled-ontology-10#Task:Medical_examination"/>
        <untitled-ontology-10:taskIsFollowedBy rdf:resource="http://www.semanticweb.org/maxsp/ontologies/2023/11/untitled-ontology-10#Task:Pre-operative_Counselling_and_Consent"/>
        <untitled-ontology-10:taskNeedsQualification rdf:resource="http://www.semanticweb.org/maxsp/ontologies/2023/11/untitled-ontology-10#Qualification:Nurse"/>
        <untitled-ontology-10:taskNeedsResource rdf:resource="http://www.semanticweb.org/maxsp/ontologies/2023/11/untitled-ontology-10#ResourceType:AllergyDetails"/>
        <untitled-ontology-10:taskNeedsResource rdf:resource="http://www.semanticweb.org/maxsp/ontologies/2023/11/untitled-ontology-10#ResourceType:Patients_file"/>
        <untitled-ontology-10:taskNeedsResource rdf:resource="http://www.semanticweb.org/maxsp/ontologies/2023/11/untitled-ontology-10#ResourceType:Present_medications"/>
        <untitled-ontology-10:taskHasName>Reviewing Patient&apos;s health History</untitled-ontology-10:taskHasName>
        <untitled-ontology-10:taskHasTimeNeeded rdf:datatype="http://www.w3.org/2001/XMLSchema#decimal">10</untitled-ontology-10:taskHasTimeNeeded>
        <untitled-ontology-10:taskPriority rdf:datatype="http://www.w3.org/2001/XMLSchema#decimal">1</untitled-ontology-10:taskPriority>
    </owl:NamedIndividual>
    


    <!-- http://www.semanticweb.org/maxsp/ontologies/2023/11/untitled-ontology-10#Workflow:PatientStuff -->

    <owl:NamedIndividual rdf:about="http://www.semanticweb.org/maxsp/ontologies/2023/11/untitled-ontology-10#Workflow:PatientStuff">
        <rdf:type rdf:resource="http://www.semanticweb.org/maxsp/ontologies/2023/11/untitled-ontology-10#workflow"/>
        <untitled-ontology-10:startTaskIs rdf:resource="http://www.semanticweb.org/maxsp/ontologies/2023/11/untitled-ontology-10#Task:Medical_examination"/>
        <untitled-ontology-10:workflowHasName>workflow one</untitled-ontology-10:workflowHasName>
    </owl:NamedIndividual>
    


    <!-- 
    ///////////////////////////////////////////////////////////////////////////////////////
    //
    // Annotations
    //
    ///////////////////////////////////////////////////////////////////////////////////////
     -->

    <rdf:Description rdf:about="http://www.semanticweb.org/maxsp/ontologies/2023/11/untitled-ontology-10#interarrivalTime">
        <rdfs:comment>some idea for the future, there may be a specification along this proerty as kind of sim setting, such that you dont have to model the simtime where events occur. instead u pass some functionthat is used to calculate some sort of interarrival time


yet there is no implementeation for this</rdfs:comment>
    </rdf:Description>
</rdf:RDF>



<!-- Generated by the OWL API (version 4.5.25.2023-02-15T19:15:49Z) https://github.com/owlcs/owlapi -->

